src/3d/Options.fsti
@@ -30,6 +30,10 @@ val get_skip_c_makefiles : unit -> ML bool
 
 val get_no_everparse_h : unit -> ML bool
 
+val get_hoist_locals : unit -> ML bool
+
+val get_init_locals : unit -> ML (option string)
+
 val get_check_hashes : unit -> ML (option check_hashes_t)
 
 val get_save_hashes : unit -> ML bool
